

#  Three line summary

-   The spectrum can be thought of heuristically as the frequencies that
    represent an element of a Banach algebra
    [test](https://nowheredifferentiable.com/2023-01-29-PDE-1/#:~:text=the%20Fourier%20transform-,The,-study%20of%20the).
    Cite me 2 (\ref{e2})  and
    mr murhp [1](https://link.springer.com/book/10.1007/978-1-4612-0949-2) and someone else [2](https://www.dcs.warwick.ac.uk/~feng/papers/Random\U Fields\U and\U Geometry\U %5BAdler%5D.pdf).

-   In a unital Banach algebra every element has non-empty spectrum.

-   A commutative Banach algebra $A$ can be thought of as a subgroup of
    continuous functions.

# Why should I care?

We introduce the basis of spectral theory which is useful to \...

# Preliminary definitions

Here I include all the needed definitions. Many of them will be familiar
if the reader has an algebra background and can be skimmed over.


**Definition 1**. An algebra $A$ is a vector space together with a
multiplication which is bilinear and associative. That is,


<div>
 $$\begin{aligned}
			(a+b)c=ac+bc;\quad a(b+c)=ab+ac; \quad a(bc)=(ab)c \forall a,b,c \in A.

\end{aligned}$$
</div>

  Note that in general we do not require that the product
is commutative. Though this will be a common requirement later on. We
will take $A$ for the remainder to be a vectro space over $\mathbb{C}$



**Definition 2**. Given a norm $\lVert \cdot  \rVert$ on algebra $A$ we
say that $(A, \lVert  \rVert)$ is a normed algebra if the norm is
submultiplicative. That is,

<div>
 $$\begin{aligned}
			\lVert ab \rVert\leq \lVert a \rVert\lVert b \rVert.

\end{aligned}$$
</div>





**Definition 3**. We say that a normed algebra
$(A,\lVert \cdot  \rVert)$ is a Banach algebra if it is complete. We
say that it is unital if there exists an identity $1$ for the
multiplication

<div>
 $$\begin{align}
\label{e3}
			a 1=1 a, \quad\forall a\in A.

\end{align}$$
</div>



and we say that it is commutative if

<div>
 $$\begin{aligned}
			ab= ba , \quad\forall a,b \in A.

\end{aligned}$$
</div>





**Definition 4**. Given $a \in  A$ we say that
$\lambda  \in \mathbb{C}$ is in the spectrum of $a$ if $\lambda 1-a$
is not invertible. We write $\sigma (a) \subset \mathbb{C}$ for the
set of such $\lambda$.



**Definition 5**. Given two algebras $A,B$ we say that
$\varphi: A\to B$ is a homomorphism if it is linear and respects the
product. That is,

<div>
 $$\begin{aligned}
			\varphi(a+ \lambda b)= \varphi(a)+ \lambda  \varphi(b);\quad \varphi(ab)=\varphi(a) \varphi(b) , \quad\forall a ,b \in  A.

\end{aligned}$$
</div>

  If $A,B$ are unital and $\varphi(1)=1$ we say that
$\varphi$ is unital. If $\varphi$ has an inverse $\varphi$ and
$\varphi$ and $\varphi^{-1}$ are continuous we say that it is a
homeomorphism


Note that any morphism $\varphi$ between unital algebras conserves
invertability. However that, even if $A,B$ are unital it may be the case
that $\varphi(1)$ is not (consider for example the zero morphism).


Definition 6. We say that $\varphi$ is a character of $A$ if
$\varphi:A\to \mathbb{C}$ is a homomorphism.



Definition 7. Given an algebra $A$ we say that $B \subset A$ is a
sub-algebra if it is subspace of $A$ closed under multiplication. That
is $B$ itself is an algebra.



Definition 8. Given an algebra $A$, we say that $I \subset A$ is an
ideal of $A$ if $I$ is stable under multiplication with elements is
$A$. That is

<div>
 $$\begin{aligned}
			AI := \{ a b: a\in A, \quad  b \in I \} \subset I; \quad IA \subset I .

\end{aligned}$$
</div>

  We say that $I$ is maximal if given any other ideal
$J$ such that $I\subset J$ it holds that $J=A$.


We recall that, by Zorn's Lemma every algebra has a maximal ideal.


Definition 9. Given a closed ideal $I$ of an algebra $A$ we define
the quotient algebra $A/I$ to be the set of equivalence classes under
the relation

<div>
 $$\begin{aligned}
			a \sim b \iff a-b \in I.

\end{aligned}$$
</div>

  With the product
$\overline{a}\overline{b}:= \overline{ab}$ and the norm


<div>
 $$\begin{aligned}
			\lVert \overline{a} \rVert:= \inf\U { b \in  I } \lVert a+b \rVert.

\end{aligned}$$
</div>




We note that it is necessary for $I$ to be closed so that if
$\lVert \overline{a} \rVert=0$ then $a \in I$, that is $\overline{a}=0$.

# Introduction

# The big theorems

We now state the main theorems and outline the proof


**Theorem 1**. Given a unital Banach algebra $A$ it holds that

1.  The set of invertible elements in $A$ is open.

2.  Taking the inverse is smooth.

3.  $\sigma (a)$ is a closed subset of $\subset B(0,\lVert a \rVert)$



Proof. All of these facts can be proved via the Von-Neumman series for
the inverse

<div>
 $$\begin{aligned}
			(1 -a)^{-1}=\sum\U {n=0}^{\infty} a^n, \quad\forall a \in B(0,1) .

\end{aligned}$$
</div>

  ◻



**Theorem 2** (Gelfand's theorem). Given a unital Banach algebra $A$,
$\sigma (a)\neq \emptyset$ for all $a\in A$.



Proof. Suppose not, then $(\lambda 1-a)^{-1}$ exists for all
$\lambda \in  \mathbb{C}$. Let us consider the function
$f:\mathbb{C}\to \mathbb{C}$

<div>
 $$\begin{align}
\label{e1}
			f(\lambda):= (\lambda 1-a)^{-1}.

\end{align}$$
</div>

  Since taking inverse is smooth, $f$ is smooth and thus
bounded on $B(0,2\lVert a \rVert)$. Furthermore, using Neumann's series
for the inverse we obtain that

<div>
 $$\begin{aligned}
			\lVert f(\lambda ) \rVert = \left| \lambda^{-1} \right| \lVert \sum\U {n=0}^{\infty}  (a / \lambda)^n  \rVert\leq \left| \lambda \right|^{-1} \sum\U {n=0}^{\infty} (\lVert a \rVert / \lambda)^n \leq \frac{1}{\left|  \lambda  \right|}\leq \frac{1}{2 \lVert a \rVert}  .

\end{aligned}$$
</div>

  As a result $f$ is a bounded smooth function and
$\ell (f(\lambda ))$ is a bounded entire function for any
$\ell \in A^$. By Liouville's theorem $\ell (f(\lambda ))$ is constant.
Since this holds for all $\ell \in  A^$ we deduce that $f(\lambda )$ is
constant. This leads to a contradiction by taking
$\lambda =1, \lambda =0$ as we get

<div>
 $$\begin{align}
\label{e2}
			I -a= a   .

\end{align}$$
</div>

  Citing (\ref{e1})  and (\ref{e2})
and referencing [3](https://link.springer.com/book/10.1007/978-1-4612-0949-2). ◻


We now discuss Gelfand's representation theorem. First some lemmas


**Lemma 1** (Codimension of a maximal ideal is 1 ). Let $I$ be a
maximal ideal in a commutative unital Banach Algebra $A$, then
$A \simeq I+ \mathbb{C}\cdot 1$.



Proof. We must show that any $a \in A$ can be written $b+\lambda$
where $b\in I$. Given $\overline{a} \in A/I$ there exists by Gelfand's
theorem $\lambda  \in  \mathbb{C}$ such that $\overline{\lambda -a}$ is
not invertible. Since $A /I$ is a field we deduce that
$\overline{\lambda -a}=0$, that is there exists $b \in  I$ such that
$b+ \lambda =a$ as desired. ◻



**Proposition 1**. Let $A$ be a commutative Banach algebra.There is a
bijective correspondence



<div>
 $$\begin{aligned}
			\Omega(A): & \simeq \{\text{Maximal ideals } I \subset A\}  . \\
			           & \varphi    \longmapsto \text{ker}(\varphi).

\end{aligned}$$
</div>




Proof. The mapping is well defined as
$a -\varphi(a) \in \text{ker}(\varphi)$ for all $a\in  A$ so
$\text{ker}(\varphi)$ is maximal. The mapping is surjective by the
previous lemma as given a maximal ideal $I$ we have that
$A=I \oplus \mathbb{C}$ and we can define
$\varphi((a,\lambda )):= \lambda$. The mapping is injective as if
$\text{ker}\varphi\U 1=\text{ker} \varphi\U 2$ then
$\varphi\U 1(a -\varphi\U 2(a))=0$ for all $a \in  A$. ◻




**Proposition 2**. Let $A$ be a commutative Banach algebra. Then
$\lVert \varphi \rVert=1$ for every $\varphi \in A$.



Proof. We have that
$\varphi(a) \subset \sigma (a)\subset B(0,\lVert a \rVert)$ as a result
$\lVert \varphi \rVert\leq 1$. On the other hand $\varphi(1)^2=1$ proves
that $\varphi(1)=1$ (we recall that characters by definition are
non-zero). This shows that $\lVert \varphi \rVert \geq 1$ and concludes
the proof. ◻



**Theorem 3**. Given a commutative unital Banach algebra $A$ it holds
that

<div>
 $$\begin{aligned}
			\sigma (a)=\{\varphi(a): \varphi \in \Omega(A)\} .

\end{aligned}$$
</div>

  If $A$ is not unital then

<div>
 $$\begin{aligned}
			\sigma (a)=\{\varphi(a): \varphi \in \Omega(A)\} \cup \{0\}  .

\end{aligned}$$
</div>





Proof. To prove the direct inclusion consider
$\lambda \not\in \sigma (a)$, then we may take by Zorn's lemma a proper
maximal ideal $I$ with $\lambda -a \in I$. By the previous proposition
we can take $I =\text{ker} \varphi$ for some character $\varphi$, from
which we deduce that $\varphi(\lambda -a)=\lambda -\varphi(a)=0$.

The reverse inclusion is immediate from the fact that
$\varphi(a-\varphi(a))=0$ so $a- \varphi(a)$ is not invertible for any
$a \in  A$.

Suppose now $A$ is not unital, then we unitize it by considering
$\tilde{A}$ as previously. The characters of $\tilde{A}$ are
$\Omega(A) \cup \{\tau\U 0\}$ where $\tau\U 0((a,\lambda )):= \lambda$.
Applying the just prove result to $\tilde{A}$ shows that, since
$\tau\U 0(a,0)=0$

<div>
 $$\begin{aligned}
			\sigma (a):=\sigma (\tilde{a})=\{\varphi(a): \varphi \in \Omega(A)\} \cup \{0\}  .

\end{aligned}$$
</div>

  ◻


We now consider $A^$ with the weak\ topology and $\Omega(A)$ included
within it. We recall that $A^$ is Hausdorff and thus so must be
$\Omega(A)$.


**Theorem 4**. Let $A$ be an Abelian Banach algebra. Then $\Omega(A)$
is locally compact. Furthermore, if $A$ is also unital then $\Omega(A)$
is compact.



Proof. By the previous theorem we know that $\Omega(A) \subset B(0,1)$
whihc is compact with the weak star topology (Banach Aloglu's theorem).
Now, if $\varphi\U n(a) \to \varphi(a)$ for all $a \in A$ then it holds
that, by a simple argument $\varphi$ is also a morphism. Thus $\varphi$
will be a character if and only if $\varphi \neq 0$. For this reason it
is necessary to adjoin $0$ if $A$ is not unital. This shows that
$\Omega(A) \cup  \{0\}$ is closed in $B(0,1)$ and is thus compact. In
consequence $\Omega(A)$ is locally compact.

Suppose now that $A$ is unital, then we have seen than
$\lVert \varphi \rVert=1$ for all $\varphi \in  \Omega(A)$. The previous
argument shows that $\Omega(A)$ is closed (we can never reach $0$) and
as a result $\Omega(A)$ is compact. ◻


We can now identify $A$ with a sub-algebra of continuous functions on
$\Omega(A)$ via the mapping $a \to \widehat{a}$ where we define
$\widehat{a}(\varphi):= \varphi(a)$. Let us denote the image of this
mapping by $\widehat{A}$, then we obtain the following theorem


**Theorem 5** (Gelfand's represntation theorem). Let $A$ be a
commutative Banach algebra, then the mapping

<div>
 $$\begin{aligned}
			A \to\widehat{A} \subset C\U 0(\Omega(A)); \quad a\to \widehat{a}.

\end{aligned}$$
</div>

  is a norm decreasing injective homomorphism with
$\lVert \widehat{a} \rVert= r(a)$. Furhtermore, if $a$ is unital then
$\sigma (a)=\widehat{a}(\Omega(A))$ and otherwise
$\sigma (a)=\widehat{a}(\Omega(A)) \cup  \{0\}$.



Proof. To show that $\widehat{a}$ vanishes at infinity note that the
set

<div>
 $$\begin{aligned}
			\{\varphi : \widehat{a}(\varphi) \geq \epsilon \} =\widehat{a}^{-1}([\epsilon ,\lVert a \rVert]).

\end{aligned}$$
</div>

  Which is a closed subset in the compact $B(0,a)$ and
thus compact. ◻


We note however that the mapping $a \to \widehat{a}$ is in general
neither injective (this means the identification isn't prefect) not
surjective.

 example
Example 1 (Continuous Fourier Transform). Consider the Banach
Algebra $A=L^1(\mathbb{R}^d)$ with multiplication given by the
convolution

<div>
 $$\begin{aligned}
			fg(x):= \int\U {\mathbb{R}^d}f(y)g(x-y) \,\mathrm{d}y.

\end{aligned}$$
</div>

  Then the Gelfand transform can be identified with the
Fourier transform and

<div>
 $$\begin{aligned}
			\widehat{f}(\Omega)= \left\{ \widehat{f}(\omega):= \int\U {\mathbb{R}^d} f(x)e^{-2\pi i \omega \cdot  x} \,\mathrm{d}x:\omega\in \mathbb{R}^d\right\} .

\end{aligned}$$
</div>





Proof. We know that the dual of $L^1(\mathbb{R}^d)$ is
$L^\infty(\mathbb{R}^d)$. In particular every character is of the form


<div>
 $$\begin{aligned}
			\varphi\U g (f)= \int\U {\mathbb{R}^d}f \overline{g}.

\end{aligned}$$
</div>

  The condition that $\varphi\U g$ preserves multiplication
becomes by a change of variable

<div>
 $$\begin{aligned}
			g(x+y)=g(x)g(y), \quad\forall x,y \in \mathbb{R}^d.

\end{aligned}$$
</div>

  The only $g \in L^\infty (\mathbb{R}^d)$ verifying the
above are of the form $g(x)= e^{2\pi i \omega \cdot  x}$ for some
$\omega \in \mathbb{R}^d$. That is, the character group is


<div>
 $$\begin{aligned}
			\Omega(L^1(\mathbb{R}^d))\simeq\{e^{2\pi i \omega \cdot }: \omega \in \mathbb{R}^d\} .

\end{aligned}$$
</div>

  This concludes the proof (we use the abuse of notation
$\widehat{f}(\omega):=\widehat{f}(\varphi\U {e^{2\pi i \omega \cdot }})$). ◻


 example
Example 2 (Discrete Fourier Transform). Consider the Banach Algebra
$A=\ell ^\infty(\mathbb{Z}^d)$ with multiplication given by the
convolution

<div>
 $$\begin{aligned}
			gh(k):= \sum\U {k \in \mathbb{Z}^d}g(j)h(k-j) .

\end{aligned}$$
</div>

  Then the Gelfand transform can be identified with the
(inverse) Fourier transform and

<div>
 $$\begin{aligned}
			\widehat{g}(\Omega)= \left\{ \check{g}(k):= \sum\U {k \in \mathbb{Z}^d} g(x)e^{2\pi i k \cdot  x} \,\mathrm{d}x: k\in \mathbb{Z}^d\right\} .

\end{aligned}$$
</div>




Furthermore

<div>
 $$\begin{aligned}
		g(k)=\int\U {0}^1 \check{g}(k)e^{2 \pi i (j-k) \cdot x}\,\mathrm{d}x.

\end{aligned}$$
</div>




Proof. Let $e\U 1,\ldots e\U d \in A$ be defined by

<div>
 $$\begin{aligned}
			e\U n(k):= \delta \U {nk\U 1}, \quad\forall n=1,\ldots d, k\in \mathbb{Z}^d .

\end{aligned}$$
</div>

  Then we have that $A$ is generated by $e\U {1},\ldots e\U n$
with

<div>
 $$\begin{aligned}
			g(k) =\sum\U {k} g(k) e\U 1^{k\U 1}\ldots e\U d ^{k\U d} .

\end{aligned}$$
</div>

  Any character $\varphi$ is thus determined by where it
sends the $e\U n$ and they take the form

<div>
 $$\begin{aligned}
			\Omega(A)= \left\{ \varphi\U z (g):= \sum\U {k \in \mathbb{Z}^d} g(k) z^k: z \in \mathbb{T}^d  \right\} \simeq \mathbb{T}^d .

\end{aligned}$$
</div>

  Noting that
$\mathbb{T}^d= \left\{ e^{ 2\pi i x}: x \in \mathbb{R}^d \right\}$ and
defining

<div>
 $$\begin{aligned}
			\check{g}(x):= \varphi\U {e^{ 2\pi i x \cdot  }}(g)=\sum\U {k \in \mathbb{Z}^d} g(k) e^{2 \pi  i k \cdot x}.

\end{aligned}$$
</div>

  Gives the first part of the proof and using the
orthonormality trick

<div>
 $$\begin{aligned}
			\int\U {0}^1 \check{g}(x) e^{-2 \pi i k \cdot x}\,\mathrm{d}x=\sum\U {j \in \mathbb{Z}^d} g(j)  \int\U {0}^1 e^{2 \pi i (j-k) \cdot x}\,\mathrm{d}x= g(k).

\end{aligned}$$
</div>

  Gives the second. Where in the above we applied the
dominated convergence theorem. ◻


A pdf of version of this page is provided below:
<object data="/assets/blank.pdf" width="1000" height="1000" type='application/pdf'></object>
